heap.v
@@ -1,81 +1,58 @@
 Require Export ast.  
-Require Export Coq.Arith.Peano_dec. 
+Require Export Coq.Logic.FunctionalExtensionality.
 
 (*maps locations to terms and time stamps*)
-Definition heap := list TVar. 
 
-(*lookup an address in the heap*)
-Fixpoint lookup (H:heap) (l:location) :=
-  match H with
-      |(l', v, stamp)::H' => if eq_nat_dec l l'
-                            then Some (v, stamp)
-                            else lookup H' l
-      |nil => None
-  end. 
+Definition heap := location -> option (term*lock). 
 
-Fixpoint update H l (v : term) (stamp : lock) :=
-  match H with
-    | (l', v', s')::H' =>
-      if eq_nat_dec l l'
-      then (l', v, stamp) :: H'
-      else (l', v', s') :: update H' l v stamp
-    | nil => nil
-  end. 
-(*
- * If we can lookup a location in heap H, then we must 
- * still be able to find it if we extend the heap.
- *)
-Theorem lookupExtension : forall Hnew H l v S, 
-                            lookup H l  = Some(v, S) ->
-                            exists v' S', lookup (Hnew++H) l = Some(v', S'). 
+Definition emptyHeap : heap := fun _ => None. 
+
+Definition lookup (H:heap) l := H l. 
+
+Definition update H l v stamp : heap :=
+  fun l' => if eq_nat_dec l l'
+         then Some (v, stamp)
+         else H l'. 
+
+Theorem heapExt : forall (H1 H2 : heap), (forall l, H1 l = H2 l) <-> H1 = H2.
 Proof.
-  induction Hnew; intros. 
-  {simpl. exists v. exists S. assumption. }
-  {simpl. destruct a. destruct p. destruct (eq_nat_dec l l1). 
-   {subst. eauto. }
-   {eapply IHHnew in H0. invertHyp. eauto. }
-  }
-Qed.
+  intros. split.
+  {intros. eapply functional_extensionality; auto. }
+  {intros. subst. reflexivity. }
+Qed. 
 
 Theorem lookupUpdate : forall H l v lock v' lock',
                          lookup H l = Some(v', lock') -> 
                          lookup (update H l v lock) l = Some(v, lock). 
 Proof.
-  induction H; intros.
-  {simpl in *. inv H. }
-  {simpl in *. destruct a. destruct p. destruct (eq_nat_dec l l1).
-   {inv H0. simpl. destruct (eq_nat_dec l1 l1); auto. exfalso.
-    apply n. auto. }
-   {simpl in *. destruct (eq_nat_dec l l1).
-    {subst. exfalso. apply n; auto. }
-    {eapply IHlist. eauto. }
-   }
-  }
-Qed.
+  intros. unfold update. unfold lookup. destruct (PeanoNat.Nat.eq_dec l l); auto.
+  exfalso. apply n. auto.
+Qed. 
+
 
 Theorem updateUpdate : forall H l v v' lock lock',
                          update (update H l v lock) l v' lock' = update H l v' lock'.
 Proof.
-  induction H; intros; auto.
-  simpl in *. destruct a. destruct p. destruct (eq_nat_dec l n).
-  {simpl. subst. destruct (eq_nat_dec n n); auto. exfalso. apply n0; auto. }
-  {simpl. destruct (eq_nat_dec l n).
-   {contradiction. }
-   {rewrite IHlist. auto. }
-  }
-Qed.
+  intros. apply heapExt. intros. unfold update. destruct (PeanoNat.Nat.eq_dec l l0); auto.
+Qed. 
 
 Theorem updateIdempotent : forall H l v lock,
                              lookup H l  = Some(v, lock) ->
                              update H l v lock = H.
 Proof.
-  induction H; intros; auto.
-  simpl in *. destruct a. destruct p. destruct (eq_nat_dec l l1).
-  {subst. inv H0. auto. }
-  {rewrite IHlist. auto. assumption. }
+  intros H l v lock H0. apply heapExt. intros. unfold update.
+  destruct (PeanoNat.Nat.eq_dec l l0).
+  {subst. unfold lookup in H0. rewrite H0. reflexivity. }
+  {auto. }
 Qed. 
-
-
-
-
+  
+Theorem updatecomm : forall H l l' v v' lock lock',
+    l <> l' ->
+    update (update H l v lock) l' v' lock' =
+    update (update H l' v' lock') l v lock.
+Proof.
+  intros. apply heapExt. intros. unfold update.
+  destruct (PeanoNat.Nat.eq_dec l' l0); destruct (PeanoNat.Nat.eq_dec l l0); auto.
+  subst. exfalso; auto.
+Qed. 
   
