stepPreservesRewind.v
@@ -1,221 +1,483 @@
 Require Export semantics. 
- 
+   
 (*retrieve the stamp number from a heap location*)
 Definition getStamp (x : location * term * lock) :=
   match x with
       |(_,_,s) => s
-  end.  
-
-(*if location l is present in heap H, then if we extend H with some number of
-**locations, all of which have stamp C.  Then either we will get the same 
-**result when looking up in the extended heap or we will get something that 
-**has a timestamp of C*)
-Theorem lookupExtension : forall H' l v S H C, 
-                  lookup H l = Some(v, S) ->
-                  Forall (fun x : TVar => getStamp x = Unlocked C) H' ->
-                  lookup (H'++H) l = Some(v, S) \/
-                  exists S' v', lookup (H'++H) l = Some(v', S') /\
-                           S' = Unlocked C. 
+  end.   
+ 
+Theorem validInvalidStamp : forall tid S lock,
+                              validStamp tid S lock ->
+                              invalidStamp tid S lock -> False. 
 Proof.
-  induction H'; intros l v S H C HYP1 HYP2. 
-  {simpl. auto. }
-  {simpl in *. destruct a. destruct p. destruct (eq_nat_dec l l1). 
-   {right. subst. repeat econstructor. inv HYP2. auto. }
-   {inv HYP2. eapply IHH' in HYP1; eauto. }
+  intros tid S lock H H0.
+  inv H; inv H0; auto. omega.
+Qed.
+
+Inductive locked (tid : nat) : lock -> Prop :=
+|acquired : forall oldV v, locked tid (Locked tid oldV v). 
+ 
+Theorem validateNotIn : 
+  forall tid l v b v'' lock''' rv wv e0 L H lock' chkpnt HI HV,
+    Log.notIn l b L -> H l = Some(v'', lock''') -> validStamp tid rv lock''' -> 
+    @validate tid rv wv e0 b L (update H l v lock') 
+              (commit chkpnt HI HV) ->
+    exists HV', @validate tid rv wv e0 b L H (commit chkpnt (update HI l v'' lock''') HV').
+Proof.   
+  intros tid l v b v'' lock''' rv wv e0 L H lock' chkpnt HI HV H0 H1 HV2 H3.
+  remember (update H l v lock'). remember (commit chkpnt HI HV).
+  genDeps{{chkpnt; HI; HV; H; l; v; lock'; lock'''}}.
+  induction H3; intros; try solve[inv Heqv0].
+  {inv Heqv0. subst. exists H1. rewrite updateUpdate.
+   rewrite updateIdempotent. constructor. eassumption. }
+  {inv Heqv0. dependent destruction H2. eapply IHvalidate in H2; eauto. 
+   invertHyp. unfold lookup in H0. unfold update in H0. 
+   destruct (Nat.eq_dec l0 l). 
+   {subst. econstructor. econstructor; eauto. } 
+   {econstructor. econstructor; eauto. }
+  }
+  {inv Heqv0. dependent destruction H2. eapply IHvalidate in H2; eauto. 
+   invertHyp. unfold lookup in H0. unfold update in H0. 
+   destruct (Nat.eq_dec l0 l). 
+   {subst. econstructor. econstructor; eauto. } 
+   {econstructor. econstructor; eauto. }
+  }
+  {inv Heqv0. dependent destruction H1. 
+   eapply IHvalidate in H1; eauto. invertHyp. econstructor. 
+   rewrite updatecomm; auto. econstructor; eauto. unfold lookup in H0. 
+   unfold update in H0. destruct (Nat.eq_dec l0 l). contradiction. 
+   eassumption. }
+Qed. 
+
+Theorem validateIn :  
+  forall tid l v v'' rv wv e0 L H lock' chkpnt HI HV,
+    Log.In l L -> H l = Some(v'', lock') -> 
+    @validate tid rv wv e0 true L (update H l v lock') 
+              (commit chkpnt HI HV) ->
+    exists HV', @validate tid rv wv e0 true L H (commit chkpnt HI HV').
+Proof.
+  intros. dependent induction H2.
+  {dependent destruction H0. eapply IHvalidate in H0; eauto. 
+   invertHyp. unfold lookup in H4. unfold update in H4.
+   destruct (Nat.eq_dec l l0).
+   {subst. inv H4. econstructor. econstructor; eauto. }
+   {econstructor. econstructor; eauto. }
+  }
+  {dependent destruction H0.
+   {unfold lookup in H3. unfold update in H3.
+    destruct (Nat.eq_dec l0 l0). Focus 2. exfalso; eauto.
+    inv H3. eapply validateNotIn in H0; eauto. invertHyp.
+    erewrite <- updateUpdate. econstructor. econstructor; eauto. constructor. }
+   {eapply IHvalidate in H1; eauto. invertHyp. econstructor.
+    econstructor; eauto. unfold lookup in H3. unfold update in H3.
+    destruct (Nat.eq_dec l l0). contradiction. eassumption. }
   }
 Qed. 
 
-(*we can produce the same replay derivation under an extended heap, if everything
-**in the extension has a timestamp greater than the thread being replayed and is unlocked*)
-Theorem replayHeapExtension : forall H H' S e0 RS RS' WS WS' e e' C,
-                      replay H (Some(S,e0),RS,WS,e) (Some(S,e0),RS',WS',e') -> S < C ->
-                      Forall (fun x : TVar => getStamp x = Unlocked C) H' ->
-                      replay (H'++H) (Some(S,e0),RS,WS,e) (Some(S,e0),RS',WS',e'). 
+Theorem validateAcquiredLock : forall tid l v v' b rv wv e0 L L' H lock lock' chkpnt HI HV,
+    lookup H l = Some(v', lock) ->
+    acquireLock l v' tid rv L lock lock' L' -> 
+    @validate tid rv wv e0 true L' (update H l v lock') (commit chkpnt HI HV) ->
+    exists HV', @validate tid rv wv e0 b L H (commit chkpnt HI HV').
 Proof.
-  intros. dependent induction H0. 
-  {constructor. }
-  {inv H0. 
-   {eapply lookupExtension with (H':=H') in H11; eauto. inv H11.
-    {econstructor. eapply r_readStepValid; eauto. eauto. }
-    {invertHyp. econstructor. eapply r_readStepInvalid; eauto. constructor.
-     omega. eauto. }
+  intros tid l v v' b rv wv e0 L L' H lock lock' chkpnt HI HV H0 H1 H2.
+  dependent destruction H1. 
+  {eapply validateIn in H1; eauto. }
+  {dependent destruction H3. unfold update in H4. unfold lookup in H4. 
+   destruct (Nat.eq_dec l l). inv H4. 
+   eapply validateNotIn in H5; eauto. 
+   constructor. omega. exfalso; auto. }
+Qed. 
+
+Theorem abortNotIn : 
+  forall tid l v b v'' lock''' rv wv e0 L H lock' chkpnt HI,
+    Log.notIn l b L -> H l = Some(v'', lock''') -> validStamp tid rv lock''' ->
+    locked tid lock' ->
+    @validate tid rv wv e0 b L (update H l v lock') (abort chkpnt HI) ->
+    @validate tid rv wv e0 b L H (abort chkpnt (update HI l v'' lock''')).
+Proof.
+  intros. remember (update H l v lock'). remember (abort chkpnt HI).
+  genDeps{{chkpnt; HI; H; l; v; lock'}}.
+  induction H4; intros; try solve[inv Heqv0]. 
+  {inv Heqv0. dependent destruction H5. eapply validateNotIn in H5; eauto. 
+   invertHyp. unfold lookup in H0. unfold update in H0.
+   destruct (Nat.eq_dec l0 l).
+   {subst. inv H0. inv H3. inv H1. exfalso; auto. }
+   {econstructor; eauto. }
+  }
+  {inv Heqv0. dependent destruction H5. eapply validateNotIn in H5; eauto. 
+   invertHyp. unfold lookup in H0. unfold update in H0.
+   destruct (Nat.eq_dec l0 l).
+   {subst. inv H0. inv H3. inv H1. exfalso; auto. }
+   {econstructor; eauto. }
+  }
+  {dependent destruction H0.
+   {dependent destruction H1. eapply IHvalidate in H1; eauto.
+    subst. inv Heqv0. eapply readPropAbort; eauto. constructor. }
+   {inv Heqv0. dependent destruction H1. eapply IHvalidate in H1; eauto.
+    eapply readPropAbort; eauto. constructor. }
+  }
+  {dependent destruction H1. inv Heqv0. eapply IHvalidate in H5; eauto.
+   unfold lookup in H0. unfold update in H0. destruct (Nat.eq_dec l0 l).
+   contradiction. rewrite updatecomm; auto. eapply writePropAbort. auto.
+   eauto. }
+Qed.
+
+Theorem abortIn :  
+  forall tid l v v'' rv wv e0 L H lock' chkpnt HI,
+    Log.In l L -> H l = Some(v'', lock') -> 
+    @validate tid rv wv e0 true L (update H l v lock') 
+              (abort chkpnt HI) ->
+    @validate tid rv wv e0 true L H (abort chkpnt HI).
+Proof.
+  intros. dependent induction H2.
+  {dependent destruction H0. eapply validateIn in H0; eauto.
+   invertHyp. unfold lookup in H4. unfold update in H4. destruct (Nat.eq_dec l l0).
+   {subst. inv H4. econstructor; eauto. }
+   {econstructor; eauto. }
+  }
+  {dependent destruction H3. dependent destruction H0. eapply IHvalidate in H0; eauto.
+   eapply readPropAbort; eauto. constructor. }
+  {dependent destruction H0.
+   {unfold lookup in H3. unfold update in H3. destruct (Nat.eq_dec l0 l0).
+    {inv H3. eapply abortNotIn in H0; eauto. erewrite <- updateUpdate.
+     eapply writePropAbort; eauto. constructor. constructor. }
+    {exfalso; auto. }
    }
-   {econstructor. eapply r_readStepValid; eauto. eauto. }
-    {invertHyp. econstructor. eapply r_readStepInvalid; eauto. omega. eauto. }
-   }
-   {copy H8. eapply lookupExtension with (H':=H') in H0; eauto. inv H0. 
-    {econstructor. eapply r_readStepInvalid; eauto. eauto. }
-    {invertHyp. econstructor. eapply r_readStepInvalid; eauto. omega. eauto. }
-   }
-   {econstructor. eapply r_readInDomainStep; eauto. eauto. }
-   {econstructor. eapply r_writeStep; eauto. eauto. }
-   {econstructor. eapply r_atomicIdemStep; eauto. eauto. }
-   {econstructor. eapply r_betaStep; eauto. eauto. }
+   {eapply IHvalidate in H1; eauto. eapply writePropAbort; eauto.
+    unfold lookup in H3. unfold update in H3. destruct (Nat.eq_dec l l0).
+    contradiction. eauto. }
   }
 Qed. 
 
-(*Generalizes the previous theorem to thread pools*)
-Theorem poolRewindHeapExtension : forall H H' T C C', 
-                                    C' >= C -> poolRewind C H T ->
-                                    Forall (fun x : location * term * stamp => getStamp x = C) H' ->
-                                    poolRewind C' (H'++H) T.
+Theorem abortAcquiredLock : forall tid l v v' b rv wv e0 L L' H lock lock' chkpnt HI,
+    lookup H l = Some(v', lock) ->
+    acquireLock l v' tid rv L lock lock' L' -> 
+    @validate tid rv wv e0 true L' (update H l v lock') (abort chkpnt HI) ->
+    @validate tid rv wv e0 b L H (abort chkpnt HI).
 Proof.
-  intros. induction H1. 
-  {constructor. }
-  {constructor. rewrite rewindIFFReplay. eapply replayHeapExtension; eauto. 
-   rewrite <- rewindIFFReplay. auto. omega. }
-  {constructor; auto. }
+  intros. dependent destruction H1. 
+  {eapply abortIn in H2; eauto. }
+  {dependent destruction H3. dependent destruction H5.
+   unfold update in H5. unfold lookup in H5. 
+   destruct (Nat.eq_dec l l). inv H5. 
+   eapply abortNotIn in H2; eauto. constructor. auto. constructor. 
+   exfalso; auto. }
 Qed. 
 
-
-(*If the log at the end of a rewind derivation is invalid, then we can rewind
-**from the log returned from validate*)
-Theorem abortRewind : forall S L H S' e' L' e0 e,
-                        validate S L H S' (abort e' L') ->
-                        rewind H (Some (S, e0), [], e0) (Some (S, e0), L, e) ->
-                        rewind H (Some (S, e0), [], e0) (Some (S, e0), L', e'). 
+   
+Theorem rewindNewerStamp : forall S C H1 H2 b1 b2 tid e0 L1 L2 t1 t2 HI HV chkpnt,
+                             rewind H1 (txThread b1 tid S e0 L1 t1)
+                                    H2 (txThread b2 tid S e0 L2 t2) ->
+                             S < C -> @validate tid S C e0 b2 L2 H2 (commit chkpnt HI HV) ->
+                             rewind H1 (txThread b1 tid C e0 L1 t1)
+                                    H2 (txThread b2 tid C e0 L2 t2). 
 Proof.
-  intros. dependent induction H1. 
+  intros. genDeps{{C; chkpnt; HI; HV}}. dependent induction H; intros.
+  {constructor. }
+  {dependent destruction H1.
+   {(*r_readChkpnt*)
+     inv H6. econstructor. eapply IHrewind; eauto. 
+     eapply r_readChkpnt; eauto. rewrite H14 in H3. inv H3.
+     inv H17; econstructor. omega. }
+   {(*r_readNoChkpnt*)
+     dependent destruction H6. econstructor; eauto. 
+     eapply r_readNoChkpnt; eauto. transEq. invertEq.
+     inv H7; econstructor; eauto. omega. }
+   {(*r_readStepInvalid*)
+     dependent destruction H6. transEq. invertEq. exfalso.
+     eapply validInvalidStamp; eauto. }
+   { (*r_writeLocked*) 
+     copy H4. eapply validateAcquiredLock in H4; eauto. invertHyp.
+     econstructor. eapply IHrewind; eauto. 
+     eapply r_writeLocked; eauto. 
+     dependent destruction H7; econstructor; eauto. omega. }
+   {(*r_atomicIdemStep*)
+     econstructor; eauto. eapply r_atomicIdemStep; auto. }
+   {(*r_betaStep*)
+     econstructor; eauto. eapply r_betaStep; eauto. }
+  }
+Qed. 
+
+Theorem notInUpdate : forall H l v lock l',
+    (update H l v lock) l' = None ->
+    H l' = None. 
+Proof.
+  intros. unfold update in H0. destruct (Nat.eq_dec l l').
   {inv H0. }
-  {inv H2; eauto. 
-   {inv H0; eauto. apply decomposeEq in H10. subst. auto. }
-   {inv H0; eauto. eapply decomposeEq in H10. subst. auto. }
-   {inv H0. eauto. }
+  {assumption.  }
+Qed.
+
+(* `Nat.eq_dec l l'` == {l = l'} + {l <> l'}
+ * is of type `sumbool`
+ *)
+
+Ltac heapUnfold := unfold lookup; unfold update.
+
+Theorem rewindAllocSingle : forall tid H H' b1 b2 S e0 L l v L' e e',
+    H' l = None ->
+    rewind H (txThread b1 tid S e0 L e) H' (txThread b2 tid S e0 L' e') ->
+    exists H'', rewind H'' (txThread b1 tid S e0 L e) (update H' l v (Unlocked 0)) (txThread b2 tid S e0 L' e').
+Proof.
+  intros tid H H' b1 b2 S e0 L l v L' e e' H0 H1. genDeps{{l; v}}. 
+  induction H1; intros.
+  {repeat econstructor. }
+  {inv H0.
+   {copy H2. eapply IHrewind in H2. invertHyp. exists x. econstructor; eauto.
+    econstructor; eauto. destruct (eq_nat_dec l l0).
+    {subst. unfold lookup in H5. transEq. invertEq. }
+    {unfold lookup. unfold update. simplEq l l0. auto. }
+   }
+   {copy H2. eapply IHrewind in H0. invertHyp. exists x. econstructor. eauto.
+    econstructor; eauto. heapUnfold. destruct (Nat.eq_dec l l0); auto. 
+    subst. unfold lookup in *. transEq. invertEq. }
+   {copy H2. eapply IHrewind in H2. invertHyp. exists x. econstructor.
+    eauto. eapply r_readStepInvalid; eauto. destruct (Nat.eq_dec l l0); eauto. 
+    {unfold lookup in H5. subst. transEq. invertEq. }
+    {unfold lookup. unfold update. simplEq l l0. eauto. }
+   }
+   {copy H2. eapply notInUpdate in H2; eauto. eapply IHrewind in H2. invertHyp.
+    exists x. econstructor; eauto. destruct (Nat.eq_dec l l0).
+    {subst. unfold update in H0. destruct (Nat.eq_dec l0 l0). invertEq.
+     exfalso. apply n. auto. }
+    {rewrite <- updatecomm; auto. econstructor; eauto. heapUnfold. simplEq l l0.
+     auto. }
+   }
+   {eapply IHrewind in H2. invertHyp. exists x. econstructor; eauto. eapply r_atomicIdemStep; eauto. }
+   {eapply IHrewind in H2. invertHyp. exists x. econstructor; eauto. eapply r_betaStep; eauto. }
   }
 Qed. 
-
-Ltac lookupSame :=
-  match goal with
-      |H:logLookup ?L ?l = ?v, H':logLookup ?L ?l = ?v' |- _ =>
-       rewrite H in H'; inv H'
-      |A:lookup ?H ?l = ?v, B:lookup ?H ?l = ?v' |- _ =>
-       rewrite A in B; inv B
-  end. 
-
-(*the same rewind derivation can be produced with a newer stamp assuming the 
-**log is valid*)
-Theorem rewindDiffStamp : forall S C H e0 L e L' e' H' S', 
-                        rewind H (Some(S,e0), L, e) (Some(S,e0), L', e') -> C > S ->
-                        validate S L' H S' (commit H') ->
-                        rewind H (Some(C,e0), L, e) (Some(C,e0), L', e').
+  
+Theorem rewindAlloc : forall C H T l v,
+    H l = None -> 
+    poolRewind C H T -> poolRewind C (update H l v (Unlocked 0)) T. 
 Proof.
-  intros. generalize dependent H'. dependent induction H0; intros. constructor. 
-  inv H1.
-  {econstructor. Focus 2. eapply r_readStepValid; eauto. omega.  
-   eapply IHrewind; eauto. inv H3. eauto. }
-  {inv H3. lookupSame. omega. }
-  {econstructor. Focus 2. eapply r_readInDomainStep; eauto. eauto. }
-  {inv H3. econstructor. Focus 2. eapply r_writeStep; eauto. intros c. inv c. 
-   eapply IHrewind; eauto. }
-  {econstructor. Focus 2. eapply r_atomicIdemStep; eauto. intros c. inv c. eauto. }
-  {econstructor. Focus 2. eapply r_betaStep; eauto. intros c. inv c. eauto. }
+  intros C H T l v H0 H1. genDeps{{l; v}}. induction H1; intros.
+  {constructor. }
+  {eapply rewindAllocSingle in H0; eauto.  invertHyp. econstructor; eauto. }
+  {econstructor; eauto. }
 Qed. 
-
-(*rewind can always take place on a newer timestamp*)
-Theorem poolRewindWeakening : forall C C' H T,
-                                poolRewind C H T -> C' >= C ->
-                                poolRewind C' H T. 
+   
+Theorem poolRewindNewerStamp : forall C C' H T,
+    poolRewind C H T -> C' > C -> poolRewind C' H T. 
 Proof.
   intros. induction H0.
   {constructor. }
-  {constructor; auto. omega. }
-  {constructor; auto. }
+  {econstructor; eauto. omega. }
+  {econstructor; eauto. }
 Qed. 
 
-(*if a heap can be validated, then the resulting heap is an extension of the 
-**input heap*)
-Theorem validateHeapExtension : forall S H C H' L,
-                                    validate S L H C (commit H')  ->
-                                    exists H'', H' = H'' ++ H .
+   
+Theorem f_rewindNoninterference : forall C H C' H' T T' T2,
+    f_step C H T C' H' T' -> poolRewind C H T2 ->
+    poolRewind C' H' T2.
 Proof.
-  intros. dependent induction H0; eauto; try solve[exists nil; eauto].  
-  {invertHyp. exists ((l,v,S')::x). simpl. reflexivity. }
+  intros C H C' H' T T' T2 H0 H1. generalize dependent T2.
+  induction H0; intros; eauto. 
+  {(*if someone else aborts, then we can still rewind*)
+    inv H0.
+
+    
+
+   admit. }
+  {inv H0; auto.  
+   {admit. }
+  }
+  {eapply rewindAlloc; auto. }
+  {admit. }
+  {eapply poolRewindNewerStamp; eauto. }
+  {eapply poolRewindNewerStamp; eauto. }
+Admitted. 
+
+Theorem p_rewindNoninterference : forall C H C' H' T T' T2,
+    p_step C H T C' H' T' -> poolRewind C H T2 ->
+    poolRewind C' H' T2.
+Proof.
+  intros C H C' H' T T' T2 H0 H1. generalize dependent T2.
+  induction H0; intros; eauto. 
+  {inv H0. admit. }
+  {inv H0; auto.  
+   {admit. }
+  }
+  {eapply rewindAlloc; auto. }
+  {admit. }
+  {eapply poolRewindNewerStamp; eauto. }
+  {eapply poolRewindNewerStamp; eauto. }
+Admitted.     
+
+(*f_step preserves rewind*)
+Theorem f_stepRewind : forall C H T C' H' T', 
+                       f_step C H T C' H' T' -> poolRewind C H T ->
+                       poolRewind C' H' T'. 
+Proof.  
+  intros. induction H0; try solve[econstructor;econstructor; econstructor]. 
+  {inv H0. econstructor; econstructor. }
+  {inv H1. inv H0. dependent destruction H0.
+   {(*t_readStep*)
+     eapply rewindSingleInTX; eauto. econstructor. eauto.
+     eapply r_readChkpnt; eauto. }
+   {(*t_readStep*)
+     eapply rewindSingleInTX; eauto. econstructor. eauto.
+     eapply r_readNoChkpnt; eauto. }
+   {(*t_writeLocked*)
+     eapply rewindSingleInTX; eauto. econstructor. eauto.
+     eapply r_writeLocked; eauto. }
+   {(*t_atomicIdemStep*)
+     eapply rewindSingleInTX; eauto. econstructor. eauto.
+     econstructor. auto. }
+   {(*t_betaStep*)
+     eapply rewindSingleInTX; eauto. econstructor. eauto.
+     eapply r_betaStep. auto. }
+  }
+  {inv H1. constructor. auto. eapply f_rewindNoninterference; eauto. }
+  {inv H1. constructor; auto. eapply f_rewindNoninterference; eauto. }
+  {(*timestamp extension*)
+    dependent destruction H1. eapply rewindSingleInTX; eauto.
+    eapply rewindNewerStamp; eauto. }
 Qed. 
 
-(*when validating the heap, the extended portion must all have time stamp
-**equal to the write version number*)
-Theorem validateStampGE : forall H' S L H C,
-                            validate S L H C (commit (H'++H)) ->
-                            Forall (fun x => getStamp x = C) H'. 
+Theorem validateNoWrites : forall tid rv wv e0 L H chkpnt HI HV,
+    @validate tid rv wv e0 false L H (commit chkpnt HI HV) ->
+    H = HI. 
 Proof.
-  intros. dependent induction H0; auto. 
-  {destruct H'. constructor. apply lengthsEq in x. simpl in *. 
-   rewrite app_length in x. omega. }
-  {copy H0. eapply validateHeapExtension in H0. invertHyp. destruct H'. 
-   simpl in x. apply lengthsEq in x. simpl in x. rewrite app_length in x. omega.
-   constructor. inv x. auto. eapply IHvalidate; eauto. inversion x. auto. }
+  intros. dependent induction H0; auto.
 Qed. 
 
-(*version clock and heap increase monotonically under the p_step relation*)
-Theorem p_stampHeapMonotonic : forall C H T C' H' T',
-             p_step C H T C' H' T' -> 
-             C' >= C /\ (exists H'', H' = H'' ++ H /\ Forall (fun x => getStamp x = C) H''). 
+Theorem commitRewind : forall H  H0 C tid e e' e0 b L L' S HV,
+    @validate tid S C e0 b L H (commit (e', L') H0 HV) -> C > S ->
+    rewind H0 (txThread false tid S e0 NilLog e0) H (txThread b tid S e0 L e) ->
+    rewind H0 (txThread false tid C e0 NilLog e0) H0 (txThread false tid C e0 L' e'). 
 Proof.
-  intros. induction H0; try invertHyp; split; eauto; try solve[exists nil; auto]. omega.  
-  {exists [(l,v,C)]. simpl. split; auto.  }
-  {copy H0. apply validateHeapExtension in H0. invertHyp. exists x. split; auto. 
-   eapply validateStampGE in H2. auto. }
+  intros H H0 C tid e e' e0 b L L' S HV H1 H2 H3.
+  genDeps{{L'; e'; HV; C}}. dependent induction H3; intros. 
+  {inv H1. constructor. }
+  {dependent destruction H0. 
+   {dependent destruction H6. 
+    copy H8. eapply validateNoWrites in H8; eauto. subst.
+    eapply rewindNewerStamp with (C := C); eauto. apply decomposeEq in H1.
+    subst. assumption. }
+   {dependent destruction H6. eapply IHrewind; eauto. }
+   {dependent destruction H6. transEq. invertEq. exfalso.
+    eapply validInvalidStamp; eauto. }
+   {(*validWrite*)
+     eapply validateAcquiredLock in H2; eauto. invertHyp. 
+     eapply IHrewind; eauto. }
+   {eauto. }
+   {eauto. }
+  }
+Qed.
+
+(** 
+ * abortRewind
+ * If the log at the end of a rewind derivation is invalid, then we can rewind
+ * from the log returned from validate.
+ * Maybe this would be easier if we didn't distinguish between H0 and H'?  
+ * they should be the same.
+ **)
+Theorem abortRewind : forall H H0 C tid e e' e0 b L L' S,
+    @validate tid S C e0 b L H (abort (e', L') H0) -> C > S ->
+    rewind H0 (txThread false tid S e0 NilLog e0) H (txThread b tid S e0 L e) ->
+    rewind H0 (txThread false tid C e0 NilLog e0) H0 (txThread false tid C e0 L' e'). 
+Proof. 
+  intros H H0 C tid e e' e0 b L L' S H1 H2 H3.
+  dependent induction H3.
+  {dependent destruction H1. inv H0. }
+  {dependent destruction H0; eauto.
+   {dependent destruction H5.  (*r_readChkpnt*)
+    (*validChkpnt case is vacuous since it returns a commit *)
+    
+    (*invalidChkpnt: this read  is out of date, contradiction...*)
+    {transEq. invertEq. exfalso. eapply validInvalidStamp; eauto. } 
+    (*readPropAbort: this read is valid, but an earlier one is out of date, use IH*)
+    {dependent destruction H6. eapply IHrewind; eauto. }
+   } 
+   {dependent destruction H5.  (*r_readNoChkpnt*)
+    (*validRead case is vacuous since it returns a commit*)
+
+    (*invalidRead: this read is out of date, contradiction...*)
+    {transEq. invertEq. exfalso. eapply validInvalidStamp; eauto. }
+    (*readPropAbort: this read is valid, but an earlier one is out of date, use IH*)
+    {dependent destruction H6. eapply IHrewind; eauto. }
+   }
+   {dependent destruction H5.   (*r_readStepInvalid*)
+    {(*invalidRead: this read is invalid, but we don't have a checkpoint*)
+      transEq. invertEq. eapply commitRewind; eauto. }
+    {dependent destruction H6. eauto. }
+   }
+   {eapply abortAcquiredLock in H5; eauto. }
+  }
+Qed.
+
+Definition invalidHeap res :=
+  match res with
+  |commit _ H _ => H
+  |abort _ H => H
+  end. 
+
+Theorem validateRewindHeapEq : forall res b H H'' tid S  L'' e' e0 C,
+    @validate tid S C e0 b L'' H res ->
+    rewind H'' (txThread false tid S e0 NilLog e0) H (txThread b tid S e0 L'' e') ->
+    invalidHeap res = H''.
+Proof.
+  intros res b H H' tid S L'' e' e0 C H0 H1.
+  generalize dependent res. dependent induction H1; intros.
+  {dependent destruction H0; auto. inv H1. }
+  {dependent destruction H0.
+   {dependent destruction H5.
+    {eapply IHrewind in H7; eauto. }
+    {eapply IHrewind in H7; eauto. }
+    {dependent destruction H6. eapply IHrewind in H5; eauto. }
+   }
+   {dependent destruction H5.
+    {eapply IHrewind in H7; eauto. }
+    {eapply IHrewind in H7; eauto. }
+    {dependent destruction H6. eapply IHrewind in H5; eauto. }
+   }
+   {dependent destruction H5.
+    {transEq. invertEq. exfalso. eapply validInvalidStamp; eauto. }
+    {transEq. invertEq. eapply IHrewind in H7; eauto. }
+    {dependent destruction H6. eapply IHrewind in H5; eauto. }
+   }
+   {destruct res.
+    {eapply validateAcquiredLock in H4; eauto. invertHyp.
+     eapply IHrewind in H6; eauto. }
+    {eapply abortAcquiredLock in H5; eauto. }
+   }
+   {eauto. }
+   {eauto. }
+  }
 Qed. 
 
 (*p_step preserves rewind*)
 Theorem p_stepRewind : forall C H T C' H' T', 
                        p_step C H T C' H' T' -> poolRewind C H T ->
                        poolRewind C' H' T'. 
-Proof.
-  intros. induction H0; try solve[repeat econstructor]. 
-  {inv H1. inv H0; exfalso; apply H6; auto. inv H0. 
-   {destruct(lt_dec S' S). 
-    {constructor; auto. econstructor; eauto. eapply r_readStepValid; eauto. }
-    {constructor; auto. econstructor; eauto. eapply r_readStepInvalid; eauto. omega. }
-   }
-   {constructor. econstructor; eauto. eapply r_readInDomainStep; eauto. auto. }
-   {econstructor. econstructor; eauto. eapply r_writeStep; eauto. auto. }
-   {econstructor. econstructor; eauto. eapply r_atomicIdemStep; eauto. auto. }
-   {econstructor. econstructor; eauto. eapply r_betaStep; eauto. auto. }
+Proof. 
+  intros. induction H0; try solve[econstructor;econstructor; econstructor]. 
+  {(*p_abortStep*)
+    inv H0. dependent destruction H1. econstructor; eauto.
+    eapply abortRewind; eauto. eapply validateRewindHeapEq in H3; eauto.
+    subst. eauto. }
+  {inv H1. inv H0. dependent destruction H0.
+   {(*t_readStep*)
+     eapply rewindSingleInTX; eauto. econstructor. eauto.
+     eapply r_readChkpnt; eauto. }
+   {(*t_readStep*)
+     eapply rewindSingleInTX; eauto. econstructor. eauto.
+     eapply r_readNoChkpnt; eauto. }
+   {(*t_writeLocked*)
+     eapply rewindSingleInTX; eauto. econstructor. eauto.
+     eapply r_writeLocked. eauto. eauto. assumption. }
+   {(*t_atomicIdemStep*)
+     eapply rewindSingleInTX; eauto. econstructor. eauto.
+     econstructor. auto. }
+   {(*t_betaStep*)
+     eapply rewindSingleInTX; eauto. econstructor. eauto.
+     eapply r_betaStep. auto. }
   }
-  {inv H1. constructor; auto. eapply p_stampHeapMonotonic in H0. invertHyp. 
-   eapply poolRewindHeapExtension; eauto. }
-  {inv H1. constructor; auto.  eapply p_stampHeapMonotonic in H0. invertHyp. 
-   eapply poolRewindHeapExtension; eauto. }
-  {inv H1. constructor; try omega. inv H3. 
-   {copy H13. eapply abortRewind in H13; eauto. eapply validateValidate in H1. 
-    invertHyp. eapply rewindDiffStamp; eauto. }
-   {apply decomposeEq in H4. subst. eapply rewindDiffStamp; eauto. }
-  }
-  {inv H1. econstructor; try omega. copy H0. eapply abortRewind in H0; eauto.
-   eapply validateValidate in H1; eauto. invertHyp. eapply rewindDiffStamp; eauto. }
-Qed. 
-
-(*version clock and heap increase monotonically under the f_step relation*)
-Theorem f_stampHeapMonotonic : forall C H T C' H' T',
-                               f_step C H T C' H' T' -> 
-                               C' >= C /\ (exists H'', H' = H'' ++ H /\ Forall (fun x => getStamp x = C) H''). 
-Proof.
-  intros. induction H0; try invertHyp; split; eauto; try solve[exists nil; auto]. omega.  
-  {exists [(l,v,C)]. simpl. split; auto.  }
-  {copy H0. apply validateHeapExtension in H0. invertHyp. exists x. split; auto. 
-   eapply validateStampGE in H2. auto. }
-Qed. 
-
-(*f_step preserves rewind*)
-Theorem f_stepRewind : forall C H T C' H' T', 
-                       f_step C H T C' H' T' -> poolRewind C H T ->
-                       poolRewind C' H' T'. 
-Proof.
-  intros. induction H0; try solve[repeat econstructor]. 
-  {inv H1. inv H0; exfalso; apply H6; auto. inv H0. 
-   {destruct(lt_dec S' S). 
-    {constructor; auto. econstructor; eauto. eapply r_readStepValid; eauto. }
-    {constructor; auto. econstructor; eauto. eapply r_readStepInvalid; eauto. omega. }
-   }
-   {constructor. econstructor; eauto. eapply r_readInDomainStep; eauto. auto. }
-   {econstructor. econstructor; eauto. eapply r_writeStep; eauto. auto. }
-   {econstructor. econstructor; eauto. eapply r_atomicIdemStep; eauto. auto. }
-   {econstructor. econstructor; eauto. eapply r_betaStep; eauto. auto. }
-  }
-  {inv H1. constructor; auto. eapply f_stampHeapMonotonic in H0. 
-   invertHyp. eapply poolRewindHeapExtension; eauto. }
-  {inv H1. constructor; auto. eapply f_stampHeapMonotonic in H0. 
-   invertHyp. eapply poolRewindHeapExtension; eauto. }
-  {constructor. constructor. omega. }
+  {inv H1. constructor. auto. eapply p_rewindNoninterference; eauto. }
+  {inv H1. constructor. eapply p_rewindNoninterference; eauto. auto. }
+  {(*timestamp extension*)
+    dependent destruction H1. eapply rewindSingleInTX; eauto.
+    eapply rewindNewerStamp; eauto. }
 Qed. 
