partialImpliesFull.v
@@ -1,71 +1,104 @@
 Require Export stepPreservesRewind.  
 
-(*if the endpoint of a replay derivation can be validated, then the 
-**start point can be validated too*)
-Theorem replayCommit : forall S L H L' S' H' e0 e e', 
-                         replay H (Some(S,e0),L,e) (Some(S,e0),L',e') ->
-                         validate S L' H S' (commit H') -> 
-                         exists H'', validate S L H S' (commit H'').
+Theorem validateNewerStamp : forall b tid rv rv' wv e0 L H chkpnt HI HV,
+    validate tid rv wv e0 L H (commit chkpnt HI HV) -> rv' >= rv ->
+    @validate tid rv' wv e0 b L H (commit chkpnt HI HV).   
 Proof.
-  intros. dependent induction H0. 
-  {eauto. }
-  {inv H0; eauto. 
-   {eapply IHreplay in H2;[idtac|eauto|eauto]. invertHyp. inv H0. eauto. }
-   {eapply IHreplay in H2;[idtac|eauto|eauto]. invertHyp. inv H0. eauto. }
-   {eapply IHreplay in H2;[idtac|eauto|eauto]. invertHyp. inv H0. eauto. }
-  }
+  intros b tid rv rv' wv e0 L H chkpnt HI HV H0 H1.
+  remember (commit chkpnt HI HV). genDeps{{chkpnt; HI; HV; rv'}}.
+  induction H0; intros; try solve[inv Heqv]. (*not sure why dependent induction doesn't work here...*)
+  {constructor. }
+  {inv Heqv. eapply validChkpnt; eauto. inv H1; constructor; eauto.
+   omega. }
+  {inv Heqv. eapply validRead; eauto. inv H1; econstructor; eauto. omega. }
+  {inv Heqv. eapply validWrite; eauto. }
 Qed. 
 
 (*simulate a replay relation under full abort semantics as long as the endpoint
 **log is valid*)
-Theorem replayFMulti : forall H S C C' e0 L e L' S' e' H', 
-                         replay H (Some(S,e0),L,e) (Some(S,e0),L',e') ->
-                         validate S L' H S' (commit H') -> S < C ->
-                         f_multistep C' H (Single(Some(C,e0),L,e)) C' H 
-                                     (Single(Some(C,e0),L',e')). 
-Proof. 
-  intros. dependent induction H0. 
+Theorem replayFMulti : forall b b' H C C' e0 L e L' e' H' chkpnt tid HI HV, 
+                         rewind H (txThread b tid C e0 L e) H' (txThread b' tid C e0 L' e') ->
+                         validate tid C C e0 L' H' (commit chkpnt HI HV) -> 
+                         multistep_rev f_step C' H (Single(txThread b tid C e0 L e)) C' H' 
+                                     (Single(txThread b' tid C e0 L' e')). 
+Proof.
+  intros b b' H C C' e0 L e L' e' H' chkpnt tid HI HV H0 H1.
+  genDeps{{chkpnt; HI; HV; C'}}. dependent induction H0; intros.
   {constructor. }
-  {inv H0. 
-   {econstructor. eapply f_transStep. eapply t_readStep; eauto. omega. eauto. }
-   {eapply replayCommit in H1; eauto. invertHyp. inv H0. lookupSame. omega. }
-   {econstructor. eapply f_transStep. eapply t_readInDomainStep; eauto. eauto. }
-   {econstructor. eapply f_transStep. eapply t_writeStep; eauto. intros c. 
-    inv c. eauto. }
-   {econstructor. eapply f_transStep. eapply t_atomicIdemStep; eauto. intros c. 
-    inv c. eauto. }
-   {econstructor. eapply f_transStep. eapply t_betaStep; eauto. intros c. 
-    inv c. eauto. }
+  {dependent destruction H1.
+   {dependent destruction H5. econstructor. eauto. unfold f_step.
+    eapply c_transStep. econstructor; eauto. }
+   {dependent destruction H5. econstructor. eauto. unfold f_step.
+    eapply c_transStep. econstructor; eauto. }
+   {dependent destruction H5. transEq. invertEq. exfalso.
+    eapply validInvalidStamp; eauto. }
+   {eapply validateAcquiredLock in H5; eauto. invertHyp. econstructor.
+    eauto. eapply c_transStep. eapply t_writeLocked; eauto. }
+   {econstructor. eauto. eapply c_transStep. eapply t_atomicIdemStep; eauto. }
+   {econstructor. eauto. eapply c_transStep. eapply t_betaStep; eauto. }
   }
 Qed. 
 
+Ltac invertEq :=
+  match goal with
+    | H1:?a = ?b, H2:?a = ?c |- _ => rewrite H1 in H2; inv H2
+  end. 
+
+Theorem falseLogHeapsSame : forall tid rv wv e0 L H chkpnt HI HV,
+    @validate tid rv wv e0 false L H (commit chkpnt HI HV) ->
+    H = HI /\ H = HV.
+Proof.
+  intros. dependent induction H0; auto. 
+Qed. 
+  
+Theorem commitChkpnt : forall tid rv b wv e0 L H e' L' HI HV,
+    @validate tid rv wv e0 b L H (commit (e', L') HI HV) ->
+    validate tid rv wv e0 L' HI (commit (e', L') HI HI).
+Proof.
+  intros. remember (e', L'). remember (commit p HI HV).
+  genDeps{{e'; L'; HI; HV; p}}. induction H0; intros.
+  {subst. inv Heqv. constructor. }
+Admitted.
+
+
+Theorem validateValidate : forall tid rv b wv e0 L H e' L' H',
+    @validate tid rv wv e0 b L H (abort (e', L') H') ->
+    exists HV, validate tid rv wv e0 L' H' (commit (e', L') H' HV).
+Proof.
+  intros. remember (abort (e',L') H'). genDeps{{e'; L'; H'}}.
+  induction H0; intros; try solve[inv Heqv]. 
+  {(*invalidChkpnt*) inv Heqv. eapply commitChkpnt in H2; eauto. }
+  {inv Heqv. eapply commitChkpnt in H2. econstructor. eauto. }
+  {inv Heqv. eauto. }
+  {inv Heqv. assert(abort (e', L') HI = abort (e', L') HI). auto.
+   eapply IHvalidate in H2. invertHyp. Admitted. 
+
+
+
+   
 (*full abort can simulate partial abort*)
 Theorem partialImpliesFull : forall C H T C' H' T', 
                                p_step C H T C' H' T' -> poolRewind C H T ->
                                f_multistep C H T C' H' T'. 
 Proof.
   intros. induction H0.
-  {econstructor. eapply f_transStep. eauto. constructor. }
-  {inv H1. apply IHp_step in H4. apply f_multi_L. auto. }
-  {inv H1. apply IHp_step in H5. apply f_multi_R. auto. }
-  {inv H1. econstructor. eapply f_forkStep; eauto. constructor. }
-  {inv H3. 
-   {copy H12. inv H1. eapply abortRewind in H12; eauto. copy H3. 
-    eapply validateValidate in H1. invertHyp. econstructor. 
-    eapply f_eagerAbort; eauto. econstructor. eauto. 
-    rewrite rewindIFFReplay in H12. eapply replayFMulti; eauto. }
-   {inv H1. econstructor. eapply f_eagerAbort; eauto.
-    eapply validateAbortRead; eauto. rewrite rewindIFFReplay in H7. 
-    eapply decomposeEq in H4. subst. eapply replayFMulti; eauto. }
-  }
-  {inv H1. copy H0. eapply abortRewind in H1; eauto. copy H0. 
-   eapply validateValidate in H2. invertHyp. econstructor. 
-   eapply f_abortStep; eauto. rewrite rewindIFFReplay in H1. 
-   eapply replayFMulti; eauto. }
-  {econstructor. eapply f_allocStep; eauto. constructor. }
-  {econstructor. eapply f_commitStep; eauto. constructor. }
-  {econstructor. eapply f_atomicStep; eauto. constructor. }
-  {econstructor. eapply f_betaStep; eauto. constructor. }
+  {inv H0. econstructor. unfold f_step. eapply c_liftedStep.
+   eapply f_abortStep; eauto. dependent destruction H1.
+   copy H3. eapply abortRewind in H2; eauto. 
+   eapply validateRewindHeapEq in H2; eauto. subst. copy H3.
+   eapply validateValidate in H3; eauto.
+   invertHyp. eapply validateNewerStamp with (rv' := C) in H5; eauto.
+   eapply replayFMulti in H5; eauto.
+   rewrite multistep_rev_eq. eauto. omega. }
+  {econstructor. eapply c_transStep; eauto. constructor. }
+  {inv H1. eapply IHc_step in H4. eapply multi_L. eauto. } 
+  {inv H1. eapply IHc_step in H5. eapply multi_R. eauto. }
+  {econstructor. eapply c_forkStep; eauto. constructor. } 
+  {econstructor. eapply c_allocStep; eauto. constructor. }
+  {econstructor. eapply c_commitStep; eauto. constructor. }
+  {econstructor. eapply c_atomicStep; eauto. constructor. }
+  {econstructor. eapply c_betaStep; eauto. constructor. }
+  {econstructor. eapply c_tsExtend; eauto. constructor. }
 Qed. 
 
 (*generalize to multistep*)
@@ -75,8 +108,8 @@ Theorem partialImpliesFullMulti : forall C H T C' H' T',
 Proof.
   intros. induction H0. 
   {constructor. }
-  {copy H0. apply p_stepRewind in H0; auto. apply IHp_multistep in H0.
-   eapply partialImpliesFull in H3; eauto. eapply f_multi_trans; eauto. }
+  {copy H0. apply p_stepRewind in H0; auto. apply IHmultistep in H0.
+   eapply partialImpliesFull in H3; eauto. eapply multi_trans; eauto. }
 Qed. 
 
 
