tactics.v
@@ -1,4 +1,6 @@
 Require Export Coq.Logic.ProofIrrelevance. 
+Require Export Coq.Init.Datatypes.
+Require Export Coq.Arith.Peano_dec.
 
 (*General Purpose tactics*)
 Ltac inv H := inversion H; subst; clear H. 
@@ -26,9 +28,50 @@ Ltac proofsEq :=
 (*If inversion produces the same hypothesis, skip it, otherwise invert all equalities*)
 Ltac invertEq :=
   match goal with
-      |H:?a = ?b |- _ => let n := fresh
-                         in inversion H as n; match type of n with
-                                                  |?a = ?b => fail
-                                              end
-      |H:?a = ?b |- _ => inv H
+  |H:?a = ?b |- _ => let n := fresh
+                   in inversion H as n; match type of n with
+                                          |?a = ?b => fail
+                                        end
+  |H:?a = ?b |- _ => inv H
+  end.
+
+Ltac transEq :=
+  match goal with
+  |H:?a = ?b,H':?a = ?c |- _ => rewrite H in H'
+  |H:?a = ?b,H':?c = ?a |- _ => rewrite H in H'
+  |H:?a = ?b,H':?b = ?c |- _ => rewrite H in H'
+  |H:?a = ?b,H':?c = ?b |- _ => rewrite H in H'
   end. 
+
+Theorem rewriteEq : forall l l' (p : l = l'), PeanoNat.Nat.eq_dec l l' = left p. 
+Proof.
+  intros. subst. destruct (PeanoNat.Nat.eq_dec l' l'); auto. replace eq_refl with e.
+  auto. apply proof_irrelevance. exfalso. auto.
+Qed. 
+
+Theorem rewriteNeq : forall l l' (p : l <> l'), PeanoNat.Nat.eq_dec l l' = right p. 
+Proof.
+  intros. subst. destruct (PeanoNat.Nat.eq_dec l l'). contradiction.
+  replace p with n. auto. apply proof_irrelevance.
+Qed. 
+
+Theorem neqSymm : forall A (l l' : A), l <> l' <-> l' <> l.
+Proof.
+  intros. split.
+  {intro. intro. subst. auto. }
+  {intro. intro. subst. auto. }
+Qed. 
+
+Ltac simplEq l l' :=
+  match goal with
+  |H : l = l |- _ =>
+   replace (PeanoNat.Nat.eq_dec l l) with ((left H) : {l = l} + {l <> l});
+   [idtac|symmetry; apply rewriteEq]
+  |H : l <> l' |- _ =>
+   replace (PeanoNat.Nat.eq_dec l l') with ((right H) : {l = l'} + {l <> l'});
+   [idtac|symmetry; apply rewriteNeq]
+  |H : l' <> l |- _ =>
+   rewrite neqSymm in H; 
+   replace (PeanoNat.Nat.eq_dec l l') with ((right H) : {l = l'} + {l <> l'});
+   [idtac|symmetry; apply rewriteNeq]
+  end.
